Inverted Indexes completely done.

src/QueryStructure/Implementation/DataStructures/Bags/InvertedIndexBags.v
@@ -67,8 +67,8 @@ Module InvertedIndexBag (MKeys : WS) (MValues : WSfun Nat_as_OT ).
 
     Fixpoint Find_MatchingIndexes
              (Mkey : KeyMapT)
-             (MValues : ValuesMapT)
              (st : IndexSearchTermT)
+             (MValues : ValuesMapT)
     : ValuesMapT :=
       match st with
         | [ ] => MValues
@@ -76,8 +76,9 @@ Module InvertedIndexBag (MKeys : WS) (MValues : WSfun Nat_as_OT ).
           match MKeys.find i Mkey with
             | Some indexes =>
               Find_MatchingIndexes
-                Mkey (filter (fun k _ => List.In_dec eq_nat_dec k (indexes)) MValues)
-                st'
+                Mkey st'
+                (filter (fun k _ => List.In_dec eq_nat_dec k (indexes)) MValues)
+                
             | None => MValues.empty _
           end
       end.
@@ -86,7 +87,7 @@ Module InvertedIndexBag (MKeys : WS) (MValues : WSfun Nat_as_OT ).
              (it : InvertedIndexMap)
              (st : SearchTerm)
     : list TItem :=
-      let matched_items := Find_MatchingIndexes it it (fst st) in
+      let matched_items := Find_MatchingIndexes it (fst st) it in
       List.filter (ItemSearchTermMatcher (snd st))
                (List.map snd (MValues.elements matched_items)).
 
@@ -94,7 +95,7 @@ Module InvertedIndexBag (MKeys : WS) (MValues : WSfun Nat_as_OT ).
                (it : InvertedIndexMap)
                (st : SearchTerm)
     : nat :=
-      let matched_items := Find_MatchingIndexes it it (fst st) in
+      let matched_items := Find_MatchingIndexes it (fst st) it in
       fold_right (fun _ n => 1 + n)
                  0
                 (List.filter (fun item => ItemSearchTermMatcher (snd st) (snd item))
@@ -127,18 +128,18 @@ Module InvertedIndexBag (MKeys : WS) (MValues : WSfun Nat_as_OT ).
            let newKeys := List.filter (fun key : E.t =>
                                          if InA_dec E.eq_dec key oldKeys then
                                            false else true) (projection item) in
-           MKeysProperties.update             
+           MKeysProperties.update
              (* Add pointer for the old keys into the key map *)
              (MKeysProperties.update notIncludedKeys
                                      (MKeys.map (cons (NumValues it)) includedKeys))
              (* Add pointer for the new keys to the key map *)
              (fold_left (fun m k => MKeys.add k [NumValues it] m) newKeys (MKeys.empty _));
-                
+
          (* Update Value Map *)
          ValuesMap := MValues.add (NumValues it) item (ValuesMap it);
          NumValues :=  S (NumValues it) |}.
 
-    Fixpoint InvertedIndex_bdelete
+    Definition InvertedIndex_bdelete
              (it : InvertedIndexMap)
              (st : SearchTerm)
     : (list TItem) * InvertedIndexMap :=
@@ -151,7 +152,7 @@ Module InvertedIndexBag (MKeys : WS) (MValues : WSfun Nat_as_OT ).
           ValuesMap := unmatchedItems;
           NumValues :=  NumValues it |}).
 
-    Fixpoint InvertedIndex_bupdate
+    Definition InvertedIndex_bupdate
              (it : InvertedIndexMap)
              (st : SearchTerm)
              (updateTerm : UpdateTermType)
@@ -181,7 +182,7 @@ Module InvertedIndexBag (MKeys : WS) (MValues : WSfun Nat_as_OT ).
                          MKeys.MapsTo key indexes (KeyMap it)
                          /\ List.In idx indexes)
          /\ forall idx,
-             NumValues it <= idx 
+             NumValues it <= idx
              -> ~ MValues.In idx (ValuesMap it).
 
     Definition InvertedIndex_ValidUpdate (update_term : UpdateTermType) :=
@@ -223,7 +224,7 @@ Module InvertedIndexBag (MKeys : WS) (MValues : WSfun Nat_as_OT ).
         apply IHl in H1; destruct_ex; eexists; eauto.
     Qed.
 
-    Lemma inA_map : 
+    Lemma inA_map :
       forall (A B : Type) eqA eqB (f : A -> B) (l : list A) (x : A),
         Proper (eqA ==> eqB) f
         -> InA eqA x l -> InA eqB (f x) (map f l).
@@ -233,9 +234,9 @@ Module InvertedIndexBag (MKeys : WS) (MValues : WSfun Nat_as_OT ).
       - econstructor 2; eauto.
     Qed.
 
-    Lemma inA_map' : 
+    Lemma inA_map' :
       forall (A B : Type) eqA eqB (f : A -> B) (l : list A) (x : B),
-        Reflexive eqA 
+        Reflexive eqA
         -> Proper (eqA ==> eqB) f
         -> InA eqB x (map f l)
         -> exists x',
@@ -249,7 +250,7 @@ Module InvertedIndexBag (MKeys : WS) (MValues : WSfun Nat_as_OT ).
 
     Lemma FMap_fold_add_MapsTo_In
       : forall (Value : Type)
-               (l : list (MKeys.key)) (k : MKeys.key) 
+               (l : list (MKeys.key)) (k : MKeys.key)
                (v : Value) (bag' : MKeys.t Value) z,
         ~ InA E.eq k (map fst  (MKeys.elements bag'))
         -> (MKeys.MapsTo k v
@@ -345,7 +346,7 @@ Module InvertedIndexBag (MKeys : WS) (MValues : WSfun Nat_as_OT ).
             eapply inA_map with (f := fst) in H5; simpl in *;
             eauto with typeclass_instances.
     Qed.
-    
+
     Lemma InvertedIndex_binsert_Preserves_RepInv :
       binsert_Preserves_RepInv InvertedIndex_RepInv InvertedIndex_binsert.
     Proof.
@@ -452,7 +453,7 @@ Module InvertedIndexBag (MKeys : WS) (MValues : WSfun Nat_as_OT ).
             rewrite MKeysProperties.filter_iff in H; intuition; eauto.
             eexists x; rewrite H1; eauto.
             unfold Proper, respectful; intros.
-            destruct (MoreMKeysFacts.BasicProperties.F.eq_dec x0 a); 
+            destruct (MoreMKeysFacts.BasicProperties.F.eq_dec x0 a);
             destruct (MoreMKeysFacts.BasicProperties.F.eq_dec y a); eauto.
             subst.
             rewrite H2 in e; intuition.
@@ -707,7 +708,7 @@ Module InvertedIndexBag (MKeys : WS) (MValues : WSfun Nat_as_OT ).
         unfold InvertedIndex_RepInv in *;
         intro H'; destruct H' as [x H'];
         rewrite add_mapsto_iff in H'; intuition.
-        eapply (H3 (S (NumValues container))); eauto.        
+        eapply (H3 (S (NumValues container))); eauto.
         eexists; eauto.
         unfold InvertedIndex_RepInv in *;
           intro H'; destruct H' as [x H'];
@@ -718,10 +719,76 @@ Module InvertedIndexBag (MKeys : WS) (MValues : WSfun Nat_as_OT ).
         exact x0.
     Qed.
 
+    Ltac case_In_dec :=
+      match goal with
+      | H : context[in_dec ?A ?B ?C] |- _ =>
+        destruct (in_dec A B C)
+      | |- context[in_dec ?A ?B ?C] =>
+        destruct (in_dec A B C)
+      end.
+
+    Instance Proper_negb_InvertedIndex_bfind_matcher i
+      : Proper (eq ==> eq ==> eq)
+               (fun (_ : MValues.key) (e : TItem) =>
+                  negb (InvertedIndex_bfind_matcher i e)).
+    Proof.
+      unfold Proper, respectful; intros; subst; eauto.
+    Qed.
+
+    Lemma MValues_elements_in_iff:
+      forall (elt : Type) (m : MValues.t elt) (x : MValues.key),
+        MValues.In x m <->
+        (In x (map fst (MValues.elements m))).
+    Proof.
+      unfold MValues.In.
+      setoid_rewrite MoreMValuesFacts.BasicFacts.elements_mapsto_iff.
+      intros; induction (MValues.elements m); split; simpl; intros.
+      - destruct_ex; inversion H.
+      - inversion H.
+      - destruct_ex; inversion H; subst.
+        destruct H1; simpl in *; subst; eauto.
+        right; eapply IHl; eauto.
+      - inversion H; subst.
+        eexists (snd a); constructor; destruct a; split; simpl; eauto.
+        apply IHl in H0; destruct_ex; eexists; eauto.
+    Qed.
+
     Lemma InvertedIndex_bdelete_Preserves_RepInv :
       bdelete_Preserves_RepInv InvertedIndex_RepInv InvertedIndex_bdelete.
     Proof.
-    Admitted.
+      unfold bdelete_Preserves_RepInv, InvertedIndex_bdelete, InvertedIndex_RepInv; simpl.
+      intros; destruct search_term; intuition.
+      - rewrite MoreMKeysFacts.BasicFacts.map_mapsto_iff in H0;
+        destruct H0; intuition; subst; apply filter_In in H3; intuition.
+        case_In_dec; try discriminate.
+        destruct (H _ _ H5 _ H0); intuition.
+        eexists x0; split; eauto.
+        apply filter_iff; intros; eauto with typeclass_instances.
+        split; eauto.
+        rewrite <- MValues_elements_in_iff in n.
+        unfold InvertedIndex_bfind_matcher; simpl.
+        destruct (IncludedInA_dec i (projection x0)); simpl; eauto.
+        case_eq (i0 x0); intros; simpl; auto.
+        destruct n; exists x0; rewrite filter_iff; eauto with typeclass_instances.
+        intuition.
+        unfold InvertedIndex_bfind_matcher; simpl.
+        rewrite H3; destruct (IncludedInA_dec i (projection x0)); simpl; eauto.
+      - rewrite filter_iff in H0; eauto with typeclass_instances; intuition.
+        destruct (H1 _ _ H4 _ H3); intuition.
+        eexists _; split.
+        rewrite MoreMKeysFacts.BasicFacts.map_mapsto_iff.
+        eexists _; split; eauto.
+        apply filter_In; split; eauto.
+        case_In_dec; eauto.
+        rewrite <- MValues_elements_in_iff in i1; destruct i1.
+        rewrite filter_iff in H0; eauto with typeclass_instances; intuition.
+        rewrite (MoreMValuesFacts.BasicFacts.MapsTo_fun H8 H4) in *; rewrite H9 in H5;
+        discriminate.
+      - destruct H3.
+        rewrite filter_iff in H3; eauto with typeclass_instances; intuition.
+        eapply H2; eauto.
+        eexists; eauto.
+    Qed.
 
     Lemma InvertedIndex_bupdate_Preserves_RepInv :
       bupdate_Preserves_RepInv
@@ -729,7 +796,43 @@ Module InvertedIndexBag (MKeys : WS) (MValues : WSfun Nat_as_OT ).
         InvertedIndex_ValidUpdate
         InvertedIndex_bupdate.
     Proof.
-    Admitted.
+      unfold bupdate_Preserves_RepInv, InvertedIndex_bupdate, InvertedIndex_RepInv; simpl.
+      intros; destruct search_term; intuition.
+      - destruct (H _ _ H0 _ H3); intuition.
+        setoid_rewrite MValuesProperties.update_mapsto_iff.
+        setoid_rewrite MoreMValuesFacts.BasicFacts.map_mapsto_iff.
+        case_eq (InvertedIndex_bfind_matcher (i, i0) x); intros.
+        + eexists _; split.
+          right; split.
+          eexists x; split; eauto.
+          rewrite MValuesProperties.filter_iff; intuition; eauto.
+          intro H'; destruct H' as [? H'];
+          rewrite MValuesProperties.filter_iff in H'; intuition.
+          rewrite (MoreMValuesFacts.BasicFacts.MapsTo_fun H7 H5) in *; rewrite H4 in H8;
+          discriminate.
+          unfold InvertedIndex_ValidUpdate in *.
+          rewrite <- valid_update; eauto.
+        + exists x; split; eauto.
+          left; rewrite MValuesProperties.filter_iff; intuition.
+          rewrite H4; reflexivity.
+      - setoid_rewrite MValuesProperties.update_mapsto_iff in H0; intuition.
+        + rewrite MValuesProperties.filter_iff in H4; intuition.
+          destruct (H1 _ _ H0 _ H3); intuition; eauto.
+        + setoid_rewrite MoreMValuesFacts.BasicFacts.map_mapsto_iff in H0;
+          destruct_ex; intuition; subst.
+          rewrite MValuesProperties.filter_iff in H6; intuition.
+          rewrite <- valid_update in H3.
+          destruct (H1 _ _ H0 _ H3); intuition; eauto.
+      - destruct H3.
+        setoid_rewrite MValuesProperties.update_mapsto_iff in H3;
+          eauto with typeclass_instances; intuition.
+        rewrite MValuesProperties.filter_iff in H4; intuition.
+        eapply H2; unfold MValues.In; eauto.
+        setoid_rewrite MoreMValuesFacts.BasicFacts.map_mapsto_iff in H3;
+          destruct_ex; intuition; subst.
+        rewrite MValuesProperties.filter_iff in H6; intuition.
+        eapply H2; unfold MValues.In; eauto.
+    Qed.
 
     Lemma InvertedIndex_BagEnumerateEmpty :
       BagEnumerateEmpty InvertedIndex_benumerate InvertedIndex_bempty.
@@ -756,7 +859,7 @@ Module InvertedIndexBag (MKeys : WS) (MValues : WSfun Nat_as_OT ).
       unfold BagCountCorrect, InvertedIndex_bcount, InvertedIndex_bfind;
       intros.
       induction (MValues.elements
-                   (Find_MatchingIndexes container container (fst search_term)));
+                   (Find_MatchingIndexes container (fst search_term) container));
         simpl; eauto.
       find_if_inside; simpl; eauto.
     Qed.
@@ -804,6 +907,100 @@ Module InvertedIndexBag (MKeys : WS) (MValues : WSfun Nat_as_OT ).
     Qed.
 
     Lemma Find_MatchingIndexesOK_Subset
+      : forall
+        (st : IndexSearchTermT)
+        (MKey : KeyMapT)
+        (MValues : ValuesMapT)
+        item idx,
+        MValues.MapsTo idx item (Find_MatchingIndexes MKey st MValues) ->
+        MValues.MapsTo idx item MValues.
+    Proof.
+      induction st; simpl; unfold inclA; intros; intuition.
+      - case_eq (MKeys.find a MKey); intros; rewrite H0 in H.
+        + apply IHst in H.
+          rewrite MValuesProperties.filter_iff in H; intuition.
+        + apply MValues.empty_1 in H; intuition.
+    Qed.
+
+    Add Parametric Morphism MKey st
+      : (Find_MatchingIndexes MKey st)
+        with signature (MValues.Equal ==> MValues.Equal)
+          as Find_MatchingIndexes_Equal.
+    Proof.
+      unfold MValues.Equal.
+      induction st; simpl; eauto.
+      destruct (MKeys.find a MKey); eauto.
+      intros; eapply IHst.
+      intros; apply Equal_mapsto_iff.
+      setoid_rewrite Equal_mapsto_iff in H.
+      intros; rewrite !MValuesProperties.filter_iff by eauto with typeclass_instances.
+      intuition; eapply H; eauto.
+    Qed.
+
+    Lemma Equal_filter_filter 
+      : forall f g (MValues : ValuesMapT),
+        MValues.Equal (filter f (filter g MValues))
+                      (filter (fun k x => f k x && g k x) MValues).
+    Proof.
+      intros; eapply Equal_mapsto_iff.
+      intros; rewrite !MValuesProperties.filter_iff
+        by eauto with typeclass_instances.
+      intuition; destruct (f k e); destruct (g k e); eauto.
+    Qed.
+
+    Lemma Find_MatchingIndexesOK_InclA
+      : forall
+        (st : IndexSearchTermT)
+        (MKey : KeyMapT)
+        (MValues : ValuesMapT),
+        (forall key indexes,
+            MKeys.MapsTo key indexes MKey ->
+            forall idx,
+              List.In idx indexes
+              -> exists item,
+                MValues.MapsTo idx item MValues
+                /\ InA E.eq key (projection item))
+        -> forall item idx,
+        MValues.MapsTo idx item (Find_MatchingIndexes MKey st MValues) ->
+        inclA E.eq st (projection item).
+    Proof.
+      induction st; simpl; unfold inclA; intros; intuition.
+      - inversion H1.
+      - case_eq (MKeys.find a MKey); intros; rewrite H2 in H0.
+        + inversion H1; subst.
+          * rewrite H4; pose proof (Find_MatchingIndexesOK_Subset _ _ _ H0) as H'.
+            rewrite MValuesProperties.filter_iff in H'; intuition.
+            apply MKeys.find_2 in H2.
+            destruct (H _ _ H2 idx); intuition.
+            destruct (in_dec eq_nat_dec idx l); simpl in *; congruence.
+            rewrite <- (MoreMValuesFacts.BasicFacts.MapsTo_fun H7 H3); eauto.
+          * destruct (E.eq_dec x a).
+            rewrite e; pose proof (Find_MatchingIndexesOK_Subset _ _ _ H0) as H'.
+            rewrite MValuesProperties.filter_iff in H'; intuition.
+            apply MKeys.find_2 in H2.
+            destruct (H _ _ H2 idx); intuition.
+            destruct (in_dec eq_nat_dec idx l); simpl in *; congruence.
+            rewrite <- (MoreMValuesFacts.BasicFacts.MapsTo_fun H7 H3); eauto.
+            apply MKeys.find_2 in H2.
+            apply (IHst _ _ H item idx); eauto.
+            generalize H0.
+            remember (fun (k : MValues.key) (_ : TItem) => bool_of_sumbool (in_dec eq_nat_dec k l)) as f.
+            unfold not in f; setoid_rewrite <- Heqf.
+            generalize MValues f; clear; induction st; simpl; intros; eauto.
+            rewrite MValuesProperties.filter_iff in H; intuition.
+            destruct (MKeys.find a MKey); simpl in *.
+            setoid_rewrite Equal_filter_filter in H.
+            eapply (IHst _ f).
+            setoid_rewrite Equal_filter_filter.
+            eapply Equal_mapsto_iff; eauto.
+            repeat f_equiv.
+            repeat (apply functional_extensionality; intros).
+            apply andb_comm.
+            eauto.
+        + apply MValues.empty_1 in H0; intuition.
+    Qed.
+
+    Lemma Find_MatchingIndexesOK_Subset'
     : forall
         (st : IndexSearchTermT)
         (MKey : KeyMapT)
@@ -816,20 +1013,85 @@ Module InvertedIndexBag (MKeys : WS) (MValues : WSfun Nat_as_OT ).
                    MValues.MapsTo idx item MValues
                    /\ InA E.eq key (projection item))
         -> (forall idx item,
-              MValues.MapsTo idx item MValues
-              -> forall key,
-                   InA E.eq key (projection item)
-                   -> exists indexes,
-                        MKeys.MapsTo key indexes MKey
-                        /\ List.In idx indexes)
+               MValues.MapsTo idx item MValues
+               -> forall key,
+                    InA E.eq key (projection item)
+                    -> exists indexes,
+                         MKeys.MapsTo key indexes MKey
+                         /\ List.In idx indexes)
         -> forall item idx,
-        MValues.MapsTo idx item (Find_MatchingIndexes MKey MValues st) <->
-        MValues.MapsTo idx item MValues /\
-        inclA E.eq st (projection item).
+            MValues.MapsTo idx item MValues -> 
+            inclA E.eq st (projection item) ->
+            MValues.MapsTo idx item (Find_MatchingIndexes MKey st MValues).
     Proof.
-    Admitted.
-
-    Lemma Not_inclA_NIn :
+      induction st; simpl; intros; eauto.
+      case_eq (MKeys.find a MKey); intros.
+      - apply MKeys.find_2 in H3.
+        assert (InA E.eq a (projection item)) by 
+            (eapply H2; econstructor; reflexivity).
+        destruct (H0 _ _ H1 _ H4); intuition.
+        rewrite <- (MoreMKeysFacts.BasicFacts.MapsTo_fun H6 H3); eauto.
+        eapply IHst in H1; eauto.
+        revert H7 H1; clear;
+        remember (fun (k : MValues.key) (_ : TItem) => bool_of_sumbool (in_dec eq_nat_dec k x)) as f; unfold not in Heqf; rewrite <- Heqf.
+        intro.
+        assert (forall v, f idx v = true) by
+            (rewrite Heqf; destruct (in_dec eq_nat_dec idx x); simpl; eauto).
+        generalize MValues f H; clear.
+        induction st.
+        + simpl; intros.
+          rewrite MValuesProperties.filter_iff; intuition.
+        + simpl; intros.
+          destruct (MKeys.find a MKey).
+          * eapply (IHst _ f) in H1; eauto.
+            setoid_rewrite Equal_filter_filter.
+            setoid_rewrite Equal_filter_filter in H1.
+            eapply Equal_mapsto_iff; eauto.
+            repeat f_equiv.
+            repeat (apply functional_extensionality; intros).
+            apply andb_comm.
+          * eauto.
+        + unfold inclA; intros; apply H2; econstructor 2; eauto.
+      - assert (InA E.eq a (projection item)) by 
+            (eapply H2; econstructor; reflexivity).
+        destruct (H0 _ _ H1 _ H4); intuition.
+        eapply MKeys.find_1 in H6; congruence.
+    Qed.
+    
+    Lemma Find_MatchingIndexesOK_Subset_iff
+    : forall
+        (st : IndexSearchTermT)
+        (MKey : KeyMapT)
+        (MValues : ValuesMapT),
+        (forall key indexes,
+           MKeys.MapsTo key indexes MKey ->
+            forall idx,
+              List.In idx indexes
+              -> exists item,
+                   MValues.MapsTo idx item MValues
+                   /\ InA E.eq key (projection item))
+        -> (forall idx item,
+               MValues.MapsTo idx item MValues
+               -> forall key,
+                    InA E.eq key (projection item)
+                    -> exists indexes,
+                         MKeys.MapsTo key indexes MKey
+                         /\ List.In idx indexes)
+        -> forall item idx,            
+            MValues.MapsTo idx item (Find_MatchingIndexes MKey st MValues)
+            <-> MValues.MapsTo idx item MValues
+                /\ inclA E.eq st (projection item).
+    Proof.
+      repeat split; intros.
+      eapply Find_MatchingIndexesOK_Subset; eauto.
+      eapply Find_MatchingIndexesOK_InclA; eauto.
+      intuition;
+        eapply Find_MatchingIndexesOK_Subset'; eauto.
+    Qed.
+      
+      
+      
+      Lemma Not_inclA_NIn :
       forall l l',
         ~ inclA E.eq l l' ->
         exists e, InA E.eq e l /\ ~ InA E.eq e l'.
@@ -873,13 +1135,13 @@ Module InvertedIndexBag (MKeys : WS) (MValues : WSfun Nat_as_OT ).
             Proper_ItemSearchTermMatcher).
       intuition.
       - try find_if_inside; eauto.
-        eapply Find_MatchingIndexesOK_Subset; eauto.
+        eapply Find_MatchingIndexesOK_Subset_iff; eauto.
         discriminate.
       - find_if_inside; eauto; discriminate.
-      - eapply Find_MatchingIndexesOK_Subset; eauto.
+      - eapply Find_MatchingIndexesOK_Subset_iff; eauto.
       - find_if_inside; eauto.
         apply Not_inclA_NIn in n; destruct n; split_and.
-        eapply Find_MatchingIndexesOK_Subset in H3; intuition eauto.
+        eapply Find_MatchingIndexesOK_Subset_iff in H3; intuition eauto.
     Qed.
 
       Corollary InvertedIndex_BagInsertEnumerate :
@@ -894,7 +1156,7 @@ Module InvertedIndexBag (MKeys : WS) (MValues : WSfun Nat_as_OT ).
       - econstructor; simpl; eauto using MValues.elements_3w.
         intuition.
         pose proof (@MValues.elements_2 _ (ValuesMap container) (NumValues container)) .
-        apply H3; revert H H1; clear; induction (MValues.elements (ValuesMap container)); simpl; intros; inversion H; subst; eauto.
+        eapply H3; revert H H1; clear; induction (MValues.elements (ValuesMap container)); simpl; intros; inversion H; subst; eauto.
         destruct a as [k v]; eexists v; eapply H1; econstructor; simpl.
         econstructor; simpl; eauto.
       - eauto using MValues.elements_3w.
@@ -906,8 +1168,103 @@ Module InvertedIndexBag (MKeys : WS) (MValues : WSfun Nat_as_OT ).
           destruct H4; simpl in *; subst; eauto.
           destruct H4; simpl in *; subst; eauto.
           rewrite <- elements_mapsto_iff in H4; subst.
-          apply H2; eexists; eauto.
+          eapply H2; eauto; eexists; eauto.
           rewrite <- elements_mapsto_iff in H4; eauto.
+    Qed.
+
+    Lemma Permutation_elements_filter B :
+      forall (f : B -> bool) container,
+        Permutation (map snd
+                         (MValues.elements
+                            (MValuesProperties.filter (fun _ => f) container)))
+                    (map snd (List.filter (fun kv => f (snd kv))(MValues.elements container))).
+    Proof.
+      intros.
+      intros; eapply Permutation_InA_cons.
+      eapply NoDupA_filter; eapply MValues.elements_3w.
+      eapply MValues.elements_3w.
+      intros.
+      rewrite filter_InA, <- !elements_mapsto_iff, MValuesProperties.filter_iff;
+        eauto with typeclass_instances.
+      unfold Proper, respectful; intros.
+      destruct H; rewrite H0; reflexivity.
+    Qed.
+
+    Lemma Permutation_elements_map B C :
+      forall (f : B -> C) container,
+        Permutation (map snd
+                         (MValues.elements
+                            (MValues.map f container)))
+                    (map snd (List.map (fun kv => (fst kv, f (snd kv))) (MValues.elements container))).
+    Proof.
+      intros.
+      intros; eapply Permutation_InA_cons.
+      - generalize (MValues.elements_3w container).
+        induction (MValues.elements container); simpl; constructor.
+        + inversion H; subst; intro; apply H2.
+          revert H0; clear; induction l; simpl; intros; inversion H0; subst.
+          * econstructor; eapply H1.
+          * econstructor 2; eauto.
+        + inversion H; subst; eauto.
+      - eapply MValues.elements_3w.
+      - intros.
+        rewrite <- !elements_mapsto_iff, map_mapsto_iff.
+        setoid_rewrite elements_mapsto_iff.
+        induction (MValues.elements container); simpl; intuition.
+        + destruct_ex; intuition; inversion H1.
+        + inversion H.
+        + destruct_ex; intuition; subst; inversion H3; subst.
+          * simpl; econstructor 1.
+            destruct H2; split; simpl in *; f_equal; eauto.
+          * econstructor 2; eauto.
+        + simpl in *; inversion H1; subst.
+          *  eexists b; split.
+             eapply H3.
+             econstructor; destruct H3; split; simpl in *; eauto.
+          * apply H0 in H3; destruct_ex; intuition; eexists; eauto.
+    Qed.
+
+    Lemma Permutation_elements_update B :
+      forall m1 m2,
+        (forall x, InA (@MValues.eq_key _) x (MValues.elements m1)
+                   -> ~ InA (@MValues.eq_key _) x (MValues.elements m2))
+        -> Permutation (map snd
+                         (MValues.elements
+                            (MValuesProperties.update (elt := B) m1 m2)))
+                    (map snd (MValues.elements m1) ++ map snd (MValues.elements m2)).
+    Proof.
+      intros; rewrite <- map_app; apply Permutation_InA_cons.
+      eapply NoDupA_app; eauto using MValues.elements_3w with typeclass_instances.
+      eapply MValues.elements_3w.
+      intros.
+      rewrite InA_app_iff, <- !elements_mapsto_iff by (eauto with typeclass_instances).
+      rewrite MValuesProperties.update_mapsto_iff; intuition.
+      right; intuition.
+      rewrite elements_mapsto_iff in H1; eapply H with (x := (k, v)); eauto.
+      revert H1; clear; induction (MValues.elements m1); intros; inversion H1; subst; eauto.
+      destruct H0; constructor; eauto.
+      destruct H0; rewrite elements_mapsto_iff in H0; revert H0; clear;
+      induction (MValues.elements m2); intros; inversion H0; subst; eauto.
+      destruct H1; simpl in *; constructor; eauto.
+    Qed.
+
+    Lemma Permutation_filter_map_snd A B :
+      forall (f : B -> bool) (l : list (A * B)),
+        Permutation (map snd (List.filter (fun kv => f (snd kv)) l))
+                    (List.filter f (map snd l)).
+    Proof.
+      intros.
+      induction l; simpl; eauto.
+      find_if_inside; simpl; eauto.
+    Qed.
+
+    Lemma Permutation_map_snd_swap A B C:
+      forall (f : B -> C) (l : list (A * B)),
+        Permutation (map snd (map (fun kv => (fst kv, f (snd kv))) l))
+                    (map f (map snd l)).
+    Proof.
+      intros.
+      induction l; simpl; eauto.
     Qed.
 
     Lemma InvertedIndex_BagDeleteCorrect :
@@ -915,15 +1272,89 @@ Module InvertedIndexBag (MKeys : WS) (MValues : WSfun Nat_as_OT ).
                        InvertedIndex_bfind_matcher
                        InvertedIndex_benumerate InvertedIndex_bdelete.
     Proof.
-    Admitted.
+      unfold BagDeleteCorrect, InvertedIndex_bdelete, InvertedIndex_benumerate;
+      simpl in *; intros; split.
+      - rewrite Permutation_elements_filter.
+        rewrite Permutation_filter_map_snd with (f := fun v => negb (_ v)).
+        induction (MValues.elements (ValuesMap container)); simpl; eauto.
+        rewrite <- partition_filter_neq.
+        case_eq (InvertedIndex_bfind_matcher search_term (snd a)); intros; simpl in *.
+        case_eq (List.partition (InvertedIndex_bfind_matcher search_term)
+                                (map snd l)); intros; simpl; eauto.
+        case_eq (List.partition (InvertedIndex_bfind_matcher search_term)
+                                (map snd l)); intros; simpl; eauto.
+      - rewrite Permutation_elements_filter, Permutation_filter_map_snd.
+        induction (MValues.elements (ValuesMap container)); simpl; eauto.
+        rewrite <- partition_filter_eq.
+        case_eq (InvertedIndex_bfind_matcher search_term (snd a)); intros; simpl in *.
+        case_eq (List.partition (InvertedIndex_bfind_matcher search_term)
+                                (map snd l)); intros; simpl; eauto.
+        case_eq (List.partition (InvertedIndex_bfind_matcher search_term)
+                                (map snd l)); intros; simpl; eauto.
+    Qed.
 
-    Lemma InvertedIndex_BagUpdateCorrect :
+    Lemma InA_eq_key_eq_key_elt
+      : forall k t l,
+        InA (MValues.eq_key (elt:=TItem)) (k, t) l <->
+        exists v, InA (@MValues.eq_key_elt _) (k, v) l.
+    Proof.
+      induction l; simpl; split; intros.
+      - inversion H.
+      - destruct_ex; inversion H.
+      - inversion H; subst.
+        + exists (snd a); destruct a; econstructor; simpl in *.
+          split; simpl; eauto.
+        + rewrite IHl in H1; destruct_ex;
+          eexists; econstructor 2; eauto.
+      - destruct_ex; inversion H; subst.
+        + constructor; apply H1.
+        + econstructor 2; apply IHl; eauto.
+    Qed.
+
+      Lemma InvertedIndex_BagUpdateCorrect :
       BagUpdateCorrect InvertedIndex_RepInv InvertedIndex_ValidUpdate
                        InvertedIndex_bfind InvertedIndex_bfind_matcher
                        InvertedIndex_benumerate
                        bupdate_transform InvertedIndex_bupdate.
     Proof.
-    Admitted.
+      unfold BagUpdateCorrect, InvertedIndex_bupdate, InvertedIndex_benumerate;
+      simpl in *; intros; split.
+      - rewrite Permutation_elements_update, Permutation_elements_filter,
+        Permutation_filter_map_snd with (f := fun v => negb (_ v)).
+        rewrite Permutation_app_swap.
+        f_equiv.
+        + induction (MValues.elements (ValuesMap container)); simpl; eauto.
+          rewrite <- partition_filter_neq.
+          case_eq (InvertedIndex_bfind_matcher search_term (snd a)); intros; simpl in *.
+          case_eq (List.partition (InvertedIndex_bfind_matcher search_term)
+                                  (map snd l)); intros; simpl; eauto.
+          case_eq (List.partition (InvertedIndex_bfind_matcher search_term)
+                                  (map snd l)); intros; simpl; eauto.
+        + rewrite Permutation_elements_map, Permutation_map_snd_swap,
+          Permutation_elements_filter, Permutation_filter_map_snd.
+          induction (MValues.elements (ValuesMap container)); simpl; eauto.
+          rewrite <- partition_filter_eq.
+          case_eq (InvertedIndex_bfind_matcher search_term (snd a)); intros; simpl in *.
+          case_eq (List.partition (InvertedIndex_bfind_matcher search_term)
+                                  (map snd l)); intros; simpl; eauto.
+          case_eq (List.partition (InvertedIndex_bfind_matcher search_term)
+                                  (map snd l)); intros; simpl; eauto.
+        + intros; destruct x.
+          intro; rewrite InA_eq_key_eq_key_elt in *; destruct_ex.
+          rewrite <- !elements_mapsto_iff in *.
+          rewrite !map_mapsto_iff in *; destruct_ex; intuition; subst.
+          rewrite filter_iff in *; intuition eauto with typeclass_instances.
+          rewrite <- (MoreMValuesFacts.BasicFacts.MapsTo_fun H H0) in H3.
+          rewrite H3 in H1; discriminate.
+      - rewrite Permutation_elements_filter, Permutation_filter_map_snd.
+        induction (MValues.elements (ValuesMap container)); simpl; eauto.
+        rewrite <- partition_filter_eq.
+        case_eq (InvertedIndex_bfind_matcher search_term (snd a)); intros; simpl in *.
+        case_eq (List.partition (InvertedIndex_bfind_matcher search_term)
+                                (map snd l)); intros; simpl; eauto.
+        case_eq (List.partition (InvertedIndex_bfind_matcher search_term)
+                                (map snd l)); intros; simpl; eauto.
+    Qed.
 
   End InvertedIndexBagDefinitions.
 
